theories/glogic.v
@@ -1,555 +1,527 @@
 Require Export g_stlc.
-Require Import sets.
+Require sets.
+From stdpp Require Import listset.
+Export GStlcTheories.
+Import sets.
 
 
 (*************************)
 (** * G Logic Deductions *)
 (*************************)
 
-Module Type SQ_SET.
-  Import GStlc.
+Module Type TM_SET.
+  Parameter tm_set : Set.
+  Declare Instance tm_set_elem_of : ElemOf tm tm_set.
+  Declare Instance tm_set_empty : Empty tm_set.
+  Declare Instance tm_set_singleton : Singleton tm tm_set.
+  Declare Instance tm_set_union : Union tm_set.
+  Declare Instance tm_set_semi_set : SemiSet _ tm_set.
+  Parameter tm_set_map : (tm -> tm) -> tm_set -> tm_set.
+  Axiom tm_set_map_spec :
+    forall f s t, t ∈ tm_set_map f s <-> exists a, a ∈ s /\ t = f a.
+End TM_SET.
 
-  Parameter sq_set : Set.
-  Declare Instance sq_set_elem_of : ElemOf tm sq_set.
-  Declare Instance sq_set_empty : Empty sq_set.
-  Declare Instance sq_set_singleton : Singleton tm sq_set.
-  Declare Instance sq_set_union : Union sq_set.
-  Declare Instance sq_set_semi_set : SemiSet _ sq_set.
-  Parameter sq_set_map : (tm -> tm) -> sq_set -> sq_set.
-  Axiom sq_set_map_spec :
-    forall f s t, t ∈ sq_set_map f s <-> exists a, a ∈ s /\ t = f a.
-End SQ_SET.
+Module tm_set : TM_SET.
+  Definition tm_set := listset tm.
+  Instance tm_set_elem_of : ElemOf tm tm_set := listset_elem_of.
+  Instance tm_set_empty : Empty tm_set := listset_empty.
+  Instance tm_set_singleton : Singleton tm tm_set := listset_singleton.
+  Instance tm_set_union : Union tm_set := listset_union.
+  Instance tm_set_semi_set : SemiSet _ tm_set := listset_simple_set.
+  Definition tm_set_map : (tm -> tm) -> tm_set -> tm_set := listset_fmap _ _.
 
-
-Module GLogic (SqSet : SQ_SET).
-  Export SqSet.
-  Export GStlcTheories.
-
-  Notation is_form C t := (has_type C t ty_prp).
-  Definition wf_sq_set C (l : sq_set) := forall t, t ∈ l -> is_form C t.
-
-  Definition wf_sequent C (p : sq_set) c := wf_sq_set C p /\ is_form C c.
-
-  Instance wf_sequent_Proper : Proper ((=) ==> (≡) ==> (=) ==> iff) wf_sequent.
+  Theorem tm_set_map_spec :
+    forall f s t, t ∈ tm_set_map f s <-> exists a, a ∈ s /\ t = f a.
   Proof.
-    intros C ? <- p q E c ? <-.
-    unfold wf_sequent, wf_sq_set. intuition; set_solver.
+    intros. unfold tm_set_map. split.
+    - intros. apply elem_of_fmap in H as [x]. exists x. intuition.
+    - intros [x]. apply elem_of_fmap. exists x. intuition.
   Qed.
+End tm_set.
+
+Export tm_set.
 
 
-  (***********************)
-  (** ** Deduction rules *)
-  (***********************)
+Notation is_form C t := (has_type C t ty_prp).
+Definition wf_tm_set C (l : tm_set) := forall t, t ∈ l -> is_form C t.
 
-  Notation "∅" := empty (in custom stlc_ty) : stlc_scope.
-  Notation "∅" := empty (in custom stlc_tm) : stlc_scope.
-  Notation "∅" := empty : stdpp_scope.
-  Infix "∪" := union (in custom stlc_tm at level 50) : stlc_scope.
-  Infix "∪" := union : stdpp_scope.
-  Notation "s +; x" := (s ∪ {[x]}) (in custom stlc_tm at level 50, left associativity) : stlc_scope.
-  Notation "s +; x" := (s ∪ {[x]}) (at level 50, left associativity) : stlc_scope.
-  Notation "{[ x ]}" := (singleton x) (in custom stlc_tm) : stlc_scope.
-  Notation "{[ x ]}" := (singleton x) : stdpp_scope.
+Definition wf_sequent C (p : tm_set) c := wf_tm_set C p /\ is_form C c.
+
+Instance wf_sequent_Proper : Proper ((=) ==> (≡) ==> (=) ==> iff) wf_sequent.
+Proof.
+  intros C ? <- p q E c ? <-.
+  unfold wf_sequent, wf_tm_set. intuition; set_solver.
+Qed.
 
 
-  Inductive is_derivable_wf : context -> sq_set -> tm -> Prop :=
-    | wrl_set C l m c :
-        l ≡ m ->
-        is_derivable_wf C l c ->
-        is_derivable_wf C m c
-    | wrl_id C a b :
-        has_type C a ty_prp ->
-        has_type C b ty_prp ->
-        tm_equiv C a b ->
-        is_derivable_wf C {[a]} b
-    | wrl_cut C l m b c :
-        is_derivable_wf C l b ->
-        is_derivable_wf C (m +; b) c ->
-        is_derivable_wf C (l ∪ m) c
-    | wrl_cL C l b c :
-        is_derivable_wf C (l +; b +; b) c ->
-        is_derivable_wf C (l +; b) c
-    | wrl_wL C l m b :
-        (forall a, a ∈ l -> has_type C a ty_prp) ->
-        is_derivable_wf C m b ->
-        is_derivable_wf C (l ∪ m) b
-    | wrl_botL C c :
-        has_type C c ty_prp ->
-        is_derivable_wf C {[gtm_bot]} c
-    | wrl_topR C :
-        is_derivable_wf C ∅ gtm_top
-    | wrl_orL C l b c d :
-        is_derivable_wf C (l +; b) c ->
-        is_derivable_wf C (l +; d) c ->
-        is_derivable_wf C (l +; <{ b \/ d }>) c
-    | wrl_orR1 C l b c :
-        has_type C c ty_prp ->
-        is_derivable_wf C l b ->
-        is_derivable_wf C l <{ b \/ c }>
-    | wrl_orR2 C l b c :
-        has_type C b ty_prp ->
-        is_derivable_wf C l c ->
-        is_derivable_wf C l <{ b \/ c }>
-    | wrl_andL1 C l b c d :
-        has_type C d ty_prp ->
-        is_derivable_wf C (l +; b) c ->
-        is_derivable_wf C (l +; <{ b /\ d }>) c
-    | wrl_andL2 C l b c d :
-        has_type C b ty_prp ->
-        is_derivable_wf C (l +; d) c ->
-        is_derivable_wf C (l +; <{ b /\ d }>) c
-    | wrl_andR C l b c :
-        is_derivable_wf C l b ->
-        is_derivable_wf C l c ->
-        is_derivable_wf C l <{ b /\ c }>
-    | wrl_impL C l b c d :
-        is_derivable_wf C l b ->
-        is_derivable_wf C (l +; d) c ->
-        is_derivable_wf C (l +; <{ b > d }>) c
-    | wrl_impR C l b c :
-        is_derivable_wf C (l +; b) c ->
-        is_derivable_wf C l <{ b > c }>
-    | wrl_forL C T l b c t :
-        has_type C t T ->
-        is_derivable_wf C (l +; subst_last C C t b) c ->
-        is_derivable_wf C (l +; <{for T, b}>) c
-    | wrl_forR C T l b sb :
-        (forall t, t ∈ sb <-> in_supp b t) ->
-        is_derivable_wf (C +: foldr ty_arr T (type_check_other <$> sb)) (sq_set_map (lift C) l) (
-          subst_last C (S C) (foldl tm_app (tm_lvl C) sb) b
-        ) ->
-        is_derivable_wf C l <{for T, b}>
-    | wrl_exL C T l b c sb :
-        (forall t, t ∈ sb <-> in_supp b t) ->
-        is_derivable_wf (C +: foldr ty_arr T (type_check_other <$> sb)) (
-          sq_set_map (lift C) l ∪
-          {[subst_last C (S C) (foldl tm_app (tm_lvl C) sb) b]}
-        ) (lift C c) ->
-        is_derivable_wf C (l +; <{ex T, b}>) c
-    | wrl_exR C T l b t :
-        has_type C t T ->
-        is_derivable_wf C l (subst_last C C t b) ->
-        is_derivable_wf C l <{ex T, b}>
-    | wrl_nabL {T b} n (_ : ~ in_supp b (gtm_nom T n)) C l c :
-      is_derivable_wf C (l +; subst_last C C (gtm_nom T n) b) c ->
-      is_derivable_wf C (l +; <{nab T, b}>) c
-    | wrl_nabR {T b} n (_ : ~ in_supp b (gtm_nom T n)) C l :
-        is_derivable_wf C l (subst_last C C (gtm_nom T n) b) ->
-        is_derivable_wf C l (<{nab T, b}>)
-  .
+(***********************)
+(** ** Deduction rules *)
+(***********************)
 
-  Inductive is_derivable : context -> sq_set -> tm -> Prop :=
-    | rl_set C l m c :
-        l ≡ m ->
-        is_derivable C l c ->
-        is_derivable C m c
-    | rl_id (C : context) l a b :
-        tm_equiv C a b ->
-        is_derivable C (l +; a) b
-    | rl_cut C l m b c :
-        has_type C b ty_prp ->
-        is_derivable C l b ->
-        is_derivable C (m +; b) c ->
-        is_derivable C (l ∪ m) c
-    | rl_cL C l b c :
-        is_derivable C (l +; b +; b) c ->
-        is_derivable C (l +; b) c
-    | rl_botL C l c :
-        is_derivable C (l +; gtm_bot) c
-    | rl_topR C l :
-        is_derivable C l gtm_top
-    | rl_orL C l b c d :
-        is_derivable C (l +; b) c ->
-        is_derivable C (l +; d) c ->
-        is_derivable C (l +; <{ b \/ d }>) c
-    | rl_orR1 C l b c :
-        is_derivable C l b ->
-        is_derivable C l <{ b \/ c }>
-    | rl_orR2 C l b c :
-        is_derivable C l c ->
-        is_derivable C l <{ b \/ c }>
-    | rl_andL1 C l b c d :
-        is_derivable C (l +; b) c ->
-        is_derivable C (l +; <{ b /\ d }>) c
-    | rl_andL2 C l b c d :
-        is_derivable C (l +; d) c ->
-        is_derivable C (l +; <{ b /\ d }>) c
-    | rl_andR C l b c :
-        is_derivable C l b ->
-        is_derivable C l c ->
-        is_derivable C l <{ b /\ c }>
-    | rl_impL C l b c d :
-        is_derivable C l b ->
-        is_derivable C (l +; d) c ->
-        is_derivable C (l +; <{ b > d }>) c
-    | rl_impR C l b c :
-        is_derivable C (l +; b) c ->
-        is_derivable C l <{ b > c }>
-    | rl_forL C T l b c t :
-        has_type C t T ->
-        is_derivable C (l +; subst_last C C t b) c ->
-        is_derivable C (l +; <{for T, b}>) c
-    | rl_forR C T l b sb :
-        (forall t, t ∈ sb <-> in_supp b t) ->
-        is_derivable (C +: foldr ty_arr T (type_check_other <$> sb)) (sq_set_map (lift C) l) (
-          subst_last C (S C) (foldl tm_app (tm_lvl C) sb) b
-        ) ->
-        is_derivable C l <{for T, b}>
-    | rl_exL C T l b c sb :
-        (forall t, t ∈ sb <-> in_supp b t) ->
-        is_derivable (C +: foldr ty_arr T (type_check_other <$> sb)) (
-          sq_set_map (lift C) l ∪
-          {[subst_last C (S C) (foldl tm_app (tm_lvl C) sb) b]}
-        ) (lift C c) ->
-        is_derivable C (l +; <{ex T, b}>) c
-    | rl_exR C T l b t :
-        has_type C t T ->
-        is_derivable C l (subst_last C C t b) ->
-        is_derivable C l <{ex T, b}>
-    | rl_nabL {T b} n (_ : ~ in_supp b (gtm_nom T n)) C l c :
-    is_derivable C (l +; subst_last C C (gtm_nom T n) b) c ->
-    is_derivable C (l +; <{nab T, b}>) c
-    | rl_nabR {T b} n (_ : ~ in_supp b (gtm_nom T n)) C l :
-        is_derivable C l (subst_last C C (gtm_nom T n) b) ->
-        is_derivable C l (<{nab T, b}>)
-  .
-
-  Notation "[{ sig ; l --> B }]" := (is_derivable sig l B)
-    (sig custom stlc_ty, l custom stlc_tm, B custom stlc_tm) : stlc_scope.
+Notation "∅" := empty (in custom stlc_ty) : stlc_scope.
+Notation "∅" := empty (in custom stlc_tm) : stlc_scope.
+Notation "∅" := empty : stdpp_scope.
+Infix "∪" := union (in custom stlc_tm at level 50) : stlc_scope.
+Infix "∪" := union : stdpp_scope.
+Notation "s +; x" := (s ∪ {[x]}) (in custom stlc_tm at level 50, left associativity) : stlc_scope.
+Notation "s +; x" := (s ∪ {[x]}) (at level 50, left associativity) : stlc_scope.
+Notation "{[ x ]}" := (singleton x) (in custom stlc_tm) : stlc_scope.
+Notation "{[ x ]}" := (singleton x) : stdpp_scope.
 
 
-  Instance is_derivable_wf_Proper :
-    Proper ((=) ==> (≡) ==> (=) ==> iff) is_derivable_wf.
-  Proof.
-    intros ? ** ? ** ? **. subst.
-    split; intros H; eapply wrl_set; try (apply H); easy.
-  Qed.
+Inductive is_derivable_wf : context -> tm_set -> tm -> Prop :=
+  | wrl_set C l m c :
+      l ≡ m ->
+      is_derivable_wf C l c ->
+      is_derivable_wf C m c
+  | wrl_id C a b :
+      has_type C a ty_prp ->
+      has_type C b ty_prp ->
+      tm_equiv C a b ->
+      is_derivable_wf C {[a]} b
+  | wrl_cut C l m b c :
+      is_derivable_wf C l b ->
+      is_derivable_wf C (m +; b) c ->
+      is_derivable_wf C (l ∪ m) c
+  | wrl_cL C l b c :
+      is_derivable_wf C (l +; b +; b) c ->
+      is_derivable_wf C (l +; b) c
+  | wrl_wL C l m b :
+      (forall a, a ∈ l -> has_type C a ty_prp) ->
+      is_derivable_wf C m b ->
+      is_derivable_wf C (l ∪ m) b
+  | wrl_botL C c :
+      has_type C c ty_prp ->
+      is_derivable_wf C {[gtm_bot]} c
+  | wrl_topR C :
+      is_derivable_wf C ∅ gtm_top
+  | wrl_orL C l b c d :
+      is_derivable_wf C (l +; b) c ->
+      is_derivable_wf C (l +; d) c ->
+      is_derivable_wf C (l +; <{ b \/ d }>) c
+  | wrl_orR1 C l b c :
+      has_type C c ty_prp ->
+      is_derivable_wf C l b ->
+      is_derivable_wf C l <{ b \/ c }>
+  | wrl_orR2 C l b c :
+      has_type C b ty_prp ->
+      is_derivable_wf C l c ->
+      is_derivable_wf C l <{ b \/ c }>
+  | wrl_andL1 C l b c d :
+      has_type C d ty_prp ->
+      is_derivable_wf C (l +; b) c ->
+      is_derivable_wf C (l +; <{ b /\ d }>) c
+  | wrl_andL2 C l b c d :
+      has_type C b ty_prp ->
+      is_derivable_wf C (l +; d) c ->
+      is_derivable_wf C (l +; <{ b /\ d }>) c
+  | wrl_andR C l b c :
+      is_derivable_wf C l b ->
+      is_derivable_wf C l c ->
+      is_derivable_wf C l <{ b /\ c }>
+  | wrl_impL C l b c d :
+      is_derivable_wf C l b ->
+      is_derivable_wf C (l +; d) c ->
+      is_derivable_wf C (l +; <{ b > d }>) c
+  | wrl_impR C l b c :
+      is_derivable_wf C (l +; b) c ->
+      is_derivable_wf C l <{ b > c }>
+  | wrl_forL C T l b c t :
+      has_type C t T ->
+      is_derivable_wf C (l +; subst_last C C t b) c ->
+      is_derivable_wf C (l +; <{for T, b}>) c
+  | wrl_forR C T l b sb :
+      (forall t, t ∈ sb <-> in_supp b t) ->
+      is_derivable_wf (C +: foldr ty_arr T (type_check_other <$> sb)) (tm_set_map (lift C) l) (
+        subst_last C (S C) (foldl tm_app (tm_lvl C) sb) b
+      ) ->
+      is_derivable_wf C l <{for T, b}>
+  | wrl_exL C T l b c sb :
+      (forall t, t ∈ sb <-> in_supp b t) ->
+      is_derivable_wf (C +: foldr ty_arr T (type_check_other <$> sb)) (
+        tm_set_map (lift C) l ∪
+        {[subst_last C (S C) (foldl tm_app (tm_lvl C) sb) b]}
+      ) (lift C c) ->
+      is_derivable_wf C (l +; <{ex T, b}>) c
+  | wrl_exR C T l b t :
+      has_type C t T ->
+      is_derivable_wf C l (subst_last C C t b) ->
+      is_derivable_wf C l <{ex T, b}>
+  | wrl_nabL {T b} n (_ : ~ in_supp b (gtm_nom T n)) C l c :
+    is_derivable_wf C (l +; subst_last C C (gtm_nom T n) b) c ->
+    is_derivable_wf C (l +; <{nab T, b}>) c
+  | wrl_nabR {T b} n (_ : ~ in_supp b (gtm_nom T n)) C l :
+      is_derivable_wf C l (subst_last C C (gtm_nom T n) b) ->
+      is_derivable_wf C l (<{nab T, b}>)
+.
 
-  Instance is_derivable_Proper :
-    Proper ((=) ==> (≡) ==> (=) ==> iff) is_derivable.
-  Proof.
-    intros ? ** ? ** ? **. subst.
-    split; intros H; eapply rl_set; try (apply H); easy.
-  Qed.
+Inductive is_derivable : context -> tm_set -> tm -> Prop :=
+  | rl_set C l m c :
+      l ≡ m ->
+      is_derivable C l c ->
+      is_derivable C m c
+  | rl_id (C : context) l a b :
+      tm_equiv C a b ->
+      is_derivable C (l +; a) b
+  | rl_cut C l m b c :
+      has_type C b ty_prp ->
+      is_derivable C l b ->
+      is_derivable C (m +; b) c ->
+      is_derivable C (l ∪ m) c
+  | rl_cL C l b c :
+      is_derivable C (l +; b +; b) c ->
+      is_derivable C (l +; b) c
+  | rl_botL C l c :
+      is_derivable C (l +; gtm_bot) c
+  | rl_topR C l :
+      is_derivable C l gtm_top
+  | rl_orL C l b c d :
+      is_derivable C (l +; b) c ->
+      is_derivable C (l +; d) c ->
+      is_derivable C (l +; <{ b \/ d }>) c
+  | rl_orR1 C l b c :
+      is_derivable C l b ->
+      is_derivable C l <{ b \/ c }>
+  | rl_orR2 C l b c :
+      is_derivable C l c ->
+      is_derivable C l <{ b \/ c }>
+  | rl_andL1 C l b c d :
+      is_derivable C (l +; b) c ->
+      is_derivable C (l +; <{ b /\ d }>) c
+  | rl_andL2 C l b c d :
+      is_derivable C (l +; d) c ->
+      is_derivable C (l +; <{ b /\ d }>) c
+  | rl_andR C l b c :
+      is_derivable C l b ->
+      is_derivable C l c ->
+      is_derivable C l <{ b /\ c }>
+  | rl_impL C l b c d :
+      is_derivable C l b ->
+      is_derivable C (l +; d) c ->
+      is_derivable C (l +; <{ b > d }>) c
+  | rl_impR C l b c :
+      is_derivable C (l +; b) c ->
+      is_derivable C l <{ b > c }>
+  | rl_forL C T l b c t :
+      has_type C t T ->
+      is_derivable C (l +; subst_last C C t b) c ->
+      is_derivable C (l +; <{for T, b}>) c
+  | rl_forR C T l b sb :
+      (forall t, t ∈ sb <-> in_supp b t) ->
+      is_derivable (C +: foldr ty_arr T (type_check_other <$> sb)) (tm_set_map (lift C) l) (
+        subst_last C (S C) (foldl tm_app (tm_lvl C) sb) b
+      ) ->
+      is_derivable C l <{for T, b}>
+  | rl_exL C T l b c sb :
+      (forall t, t ∈ sb <-> in_supp b t) ->
+      is_derivable (C +: foldr ty_arr T (type_check_other <$> sb)) (
+        tm_set_map (lift C) l ∪
+        {[subst_last C (S C) (foldl tm_app (tm_lvl C) sb) b]}
+      ) (lift C c) ->
+      is_derivable C (l +; <{ex T, b}>) c
+  | rl_exR C T l b t :
+      has_type C t T ->
+      is_derivable C l (subst_last C C t b) ->
+      is_derivable C l <{ex T, b}>
+  | rl_nabL {T b} n (_ : ~ in_supp b (gtm_nom T n)) C l c :
+  is_derivable C (l +; subst_last C C (gtm_nom T n) b) c ->
+  is_derivable C (l +; <{nab T, b}>) c
+  | rl_nabR {T b} n (_ : ~ in_supp b (gtm_nom T n)) C l :
+      is_derivable C l (subst_last C C (gtm_nom T n) b) ->
+      is_derivable C l (<{nab T, b}>)
+.
+
+Notation "[{ sig ; l --> B }]" := (is_derivable sig l B)
+  (sig custom stlc_ty, l custom stlc_tm, B custom stlc_tm) : stlc_scope.
 
 
-  Theorem has_type_fold C T h l t :
-    Forall2 (fun x X => has_type C x X) l h ->
-    has_type C t (foldr ty_arr T h) ->
-    has_type C (foldl tm_app t l) T.
-  Proof.
-    revert h t. induction l; intros h t F Ht.
-    - inversion F. now subst.
-    - simpl. destruct h; inversion F. subst.
-      eapply IHl; try eassumption.
-      has_type. now (exists t0).
-  Qed.
+Instance is_derivable_wf_Proper :
+  Proper ((=) ==> (≡) ==> (=) ==> iff) is_derivable_wf.
+Proof.
+  intros ? ** ? ** ? **. subst.
+  split; intros H; eapply wrl_set; try (apply H); easy.
+Qed.
 
-  Theorem has_type_fold2 C T sb b :
-    (forall t, t ∈ sb -> in_supp b t) ->
-    has_type (C +: foldr ty_arr T (type_check_other <$> sb)) (subst_last C (S C) (foldl tm_app (tm_lvl C) sb) b) -[ o ]- ->
-    has_type (C +: T) b ty_prp.
-  Proof.
-    intros.
-    eapply (has_type_subst_last2 _ (C +: foldr ty_arr T (type_check_other <$> sb)));
-      simpl; try eassumption; try lia.
-    - intros. now rewrite decide_True.
-    - eapply has_type_fold; has_type.
-      2:{ simpl. rewrite decide_False; ltac1:(intuition lia). }
-      remember (C +: foldr ty_arr T (type_check_other <$> sb)) as D eqn : ED.
-      clear ED H0. induction sb; simpl in *; constructor.
-      + constructor. set_unfold. eapply in_supp_other. auto.
-      + set_unfold. auto.
-  Qed.
+Instance is_derivable_Proper :
+  Proper ((=) ==> (≡) ==> (=) ==> iff) is_derivable.
+Proof.
+  intros ? ** ? ** ? **. subst.
+  split; intros H; eapply rl_set; try (apply H); easy.
+Qed.
 
-  Theorem has_type_fold2_2 C T sb b :
-    (forall t, t ∈ sb -> in_supp b t) ->
-    has_type (C +: T) b ty_prp ->
-    has_type (C +: foldr ty_arr T (type_check_other <$> sb)) (subst_last C (S C) (foldl tm_app (tm_lvl C) sb) b) -[ o ]-.
-  Proof.
-    intros.
-    eapply has_type_subst_last1.
-    - tm_simpl. lia.
-    - intros. tm_simpl. now rewrite decide_True.
-    - eapply has_type_fold; has_type.
-      2:{ simpl. rewrite decide_False; ltac1:(intuition lia). }
-      remember (C +: foldr ty_arr T (type_check_other <$> sb)) as D eqn : ED.
-      clear ED H0. induction sb; simpl in *; constructor.
-      + constructor. set_unfold. eapply in_supp_other. auto.
-      + set_unfold. auto.
-    - assumption.
-  Qed.
 
-  Theorem is_derivable_wf_wf C l c : is_derivable_wf C l c -> wf_sequent C l c.
-  Proof.
-    intros D. unfold wf_sequent. induction D; simpl in *.
-    - set_unfold. intuition. apply H0. now apply H.
-    - split; try assumption.
-      intros. set_unfold. congruence.
-    - set_unfold. intuition.
-    - set_unfold. intuition.
-    - set_unfold. intuition.
-    - set_unfold. intuition. subst. now constructor.
-    - set_unfold. intuition. now constructor.
-    - set_unfold. intuition. subst.
-      repeat (eapply ht_app); auto. now apply ht_other2.
-    - intuition. repeat (eapply ht_app); try eassumption. now apply ht_other2.
-    - intuition. repeat (eapply ht_app); try eassumption. now apply ht_other2.
-    - set_unfold. intuition. subst.
-      repeat (eapply ht_app); eauto. now apply ht_other2.
-    - set_unfold. intuition. subst.
-      repeat (eapply ht_app); eauto. now apply ht_other2.
-    - intuition. repeat (eapply ht_app); try eassumption. now apply ht_other2.
-    - set_unfold. intuition. subst.
-      repeat (eapply ht_app); eauto. now apply ht_other2.
-    - set_unfold. intuition.
-      repeat (eapply ht_app); eauto. now apply ht_other2.
-    - set_unfold. intuition. subst. econstructor.
-      + now apply ht_other2.
-      + has_type. eapply has_type_subst_last2; eauto.
-    - unfold wf_sq_set. intuition > [|econstructor].
-      + eapply has_type_lift2.
-        apply H0. apply sq_set_map_spec. eauto.
-      + now apply ht_other2.
-      + has_type. eapply has_type_fold2; try eassumption. apply H.
-    - set_unfold. intuition.
-      + eapply has_type_lift2. apply H0. left.
-        apply sq_set_map_spec. eauto.
-      + subst. econstructor > [now apply ht_other2|].
-        has_type. eapply has_type_fold2; auto. apply H.
-      + eapply has_type_lift2; eassumption.
-    - intuition. econstructor > [now apply ht_other2|].
-      has_type. eapply has_type_subst_last2; eauto.
-    - set_unfold. intuition. subst.
-      econstructor > [now apply ht_other2|].
-      has_type. eapply has_type_subst_last2; eauto.
-      now constructor.
-    - intuition. econstructor > [now apply ht_other2|].
-      has_type. eapply has_type_subst_last2; eauto.
-      now constructor.
-  Qed.
+Theorem has_type_fold C T h l t :
+  Forall2 (fun x X => has_type C x X) l h ->
+  has_type C t (foldr ty_arr T h) ->
+  has_type C (foldl tm_app t l) T.
+Proof.
+  revert h t. induction l; intros h t F Ht.
+  - inversion F. now subst.
+  - simpl. destruct h; inversion F. subst.
+    eapply IHl; try eassumption.
+    has_type. now (exists t0).
+Qed.
 
-  Theorem rl_wL C l m c :
-    [{ C; m --> c }] -> [{ C; l ∪ m --> c }].
-  Proof.
-    revert C l m c.
-    assert (MU : forall C h l, sq_set_map (lift C) <{ h ∪ l }> ≡ (sq_set_map (lift C) h) ∪ (sq_set_map (lift C) l) ). {
-      intros C h1 h2 x. set_unfold. repeat (rewrite sq_set_map_spec).
-      set_unfold. split.
-      - intros [y [Hy ->]]. destruct Hy; ltac1:(intuition eauto).
-      - intros [[y [Hy ->]] | [y [Hy ->]]]; eauto.
-    }
-    intros * H. revert l.
-    induction H; intros h; try (rewrite union_assoc in *).
-    - now rewrite <- H.
-    - now apply rl_id.
-    - eapply rl_cut; eauto.
-    - apply rl_cL. specialize IHis_derivable with h.
-      now repeat (rewrite union_assoc in *).
-    - apply rl_botL.
-    - apply rl_topR.
-    - apply rl_orL; now rewrite <- union_assoc.
-    - now apply rl_orR1.
-    - now apply rl_orR2.
-    - apply rl_andL1; now rewrite <- union_assoc.
-    - apply rl_andL2; now rewrite <- union_assoc.
-    - now apply rl_andR.
-    - apply rl_impL > [easy|]. now rewrite <- union_assoc.
-    - apply rl_impR. now rewrite <- union_assoc.
-    - eapply rl_forL > [eassumption|].
-      now rewrite <- union_assoc.
-    - eapply rl_forR; try eassumption.
-      now rewrite MU.
-    - eapply rl_exL; try eassumption.
-      now rewrite MU, <- union_assoc.
-    - eapply rl_exR; eauto.
-    - eapply rl_nabL; try eassumption.
-      now rewrite <- union_assoc.
-    - eapply rl_nabR; eauto.
-  Qed.
+Theorem has_type_fold2 C T sb b :
+  (forall t, t ∈ sb -> in_supp b t) ->
+  has_type (C +: foldr ty_arr T (type_check_other <$> sb)) (subst_last C (S C) (foldl tm_app (tm_lvl C) sb) b) -[ o ]- ->
+  has_type (C +: T) b ty_prp.
+Proof.
+  intros.
+  eapply (has_type_subst_last2 _ (C +: foldr ty_arr T (type_check_other <$> sb)));
+    simpl; try eassumption; try lia.
+  - intros. now rewrite decide_True.
+  - eapply has_type_fold; has_type.
+    2:{ simpl. rewrite decide_False; ltac1:(intuition lia). }
+    remember (C +: foldr ty_arr T (type_check_other <$> sb)) as D eqn : ED.
+    clear ED H0. induction sb; simpl in *; constructor.
+    + constructor. set_unfold. eapply in_supp_other. auto.
+    + set_unfold. auto.
+Qed.
 
-  Theorem is_derivable_wf_is_derivable C l c :
-    is_derivable_wf C l c -> [{ C; l --> c }].
-  Proof.
-    intros DW. induction DW; subst.
-    - eapply rl_set; eassumption.
-    - rewrite <- union_empty. now apply rl_id.
-    - eapply rl_cut; try eassumption.
-      apply is_derivable_wf_wf in DW1. destruct DW1. assumption.
-    - now apply rl_cL.
-    - now apply rl_wL.
-    - rewrite <- union_empty. apply rl_botL.
-    - apply rl_topR.
-    - now apply rl_orL.
-    - now apply rl_orR1.
-    - now apply rl_orR2.
-    - now apply rl_andL1.
-    - now apply rl_andL2.
-    - now apply rl_andR.
-    - now apply rl_impL.
-    - now apply rl_impR.
-    - eapply rl_forL; eassumption.
-    - eapply rl_forR; eassumption.
-    - eapply rl_exL; eassumption.
-    - eapply rl_exR; eassumption.
-    - eapply rl_nabL; eassumption.
-    - eapply rl_nabR; eassumption.
-  Qed.
+Theorem has_type_fold2_2 C T sb b :
+  (forall t, t ∈ sb -> in_supp b t) ->
+  has_type (C +: T) b ty_prp ->
+  has_type (C +: foldr ty_arr T (type_check_other <$> sb)) (subst_last C (S C) (foldl tm_app (tm_lvl C) sb) b) -[ o ]-.
+Proof.
+  intros.
+  eapply has_type_subst_last1.
+  - tm_simpl. lia.
+  - intros. tm_simpl. now rewrite decide_True.
+  - eapply has_type_fold; has_type.
+    2:{ simpl. rewrite decide_False; ltac1:(intuition lia). }
+    remember (C +: foldr ty_arr T (type_check_other <$> sb)) as D eqn : ED.
+    clear ED H0. induction sb; simpl in *; constructor.
+    + constructor. set_unfold. eapply in_supp_other. auto.
+    + set_unfold. auto.
+  - assumption.
+Qed.
 
-  Theorem is_derivable_is_derivable_wf C l c :
-    wf_sequent C l c ->  [{ C; l --> c }] -> is_derivable_wf C l c.
-  Proof.
-    intros [] D. unfold wf_sq_set in *. induction D; set_unfold.
-    - eapply wrl_set > [eassumption|].
-      apply IHD; set_solver.
-    - apply wrl_wL; try auto.
-      apply wrl_id; auto.
-    - eapply wrl_cut; first [apply IHD1 | apply IHD2]; set_solver.
-    - apply wrl_cL. apply IHD; set_solver.
-    - apply wrl_wL > [|apply wrl_botL]; set_solver.
-    - assert (E : l ≡ l ∪ ∅) > [set_solver|].
-      rewrite E. apply wrl_wL > [|apply wrl_topR].
-      clear E. set_solver.
-    - assert (is_form C <{b \/ d}>) by auto.
-      apply wrl_orL; first [apply IHD1 | apply IHD2];
-        intuition; subst; now has_type.
-    - apply wrl_orR1.
-      + now has_type.
-      + apply IHD; intuition. now has_type.
-    - apply wrl_orR2.
-      + now has_type.
-      + apply IHD; intuition. now has_type.
-    - assert (is_form C <{b /\ d}>) by auto.
-      apply wrl_andL1 > [now has_type|].
-      apply IHD; intuition. subst. now has_type.
-    - assert (is_form C <{b /\ d}>) by auto.
-      apply wrl_andL2 > [now has_type|].
-      apply IHD; intuition. subst. now has_type.
-    - assert (is_form C <{b /\ c}>) by auto. apply wrl_andR.
-      + apply IHD1. intuition. now has_type.
-      + apply IHD2. intuition. now has_type.
-    - assert (is_form C <{b > d}>) by auto. apply wrl_impL.
-      + apply IHD1. intuition. now has_type.
-      + apply IHD2; intuition. subst. now has_type.
-    - assert (is_form C <{b > c}>) by auto. apply wrl_impR.
-      apply IHD; intuition; subst; now has_type.
-    - eapply wrl_forL > [eassumption|].
-      apply IHD; intuition. subst.
-      eapply has_type_subst_last_s1 > [eassumption|].
-      assert (is_form C <{for T, b}>) by auto.
+Theorem is_derivable_wf_wf C l c : is_derivable_wf C l c -> wf_sequent C l c.
+Proof.
+  intros D. unfold wf_sequent. induction D; simpl in *.
+  - set_unfold. intuition. apply H0. now apply H.
+  - split; try assumption.
+    intros. set_unfold. congruence.
+  - set_unfold. intuition.
+  - set_unfold. intuition.
+  - set_unfold. intuition.
+  - set_unfold. intuition. subst. now constructor.
+  - set_unfold. intuition. now constructor.
+  - set_unfold. intuition. subst.
+    repeat (eapply ht_app); auto. now apply ht_other2.
+  - intuition. repeat (eapply ht_app); try eassumption. now apply ht_other2.
+  - intuition. repeat (eapply ht_app); try eassumption. now apply ht_other2.
+  - set_unfold. intuition. subst.
+    repeat (eapply ht_app); eauto. now apply ht_other2.
+  - set_unfold. intuition. subst.
+    repeat (eapply ht_app); eauto. now apply ht_other2.
+  - intuition. repeat (eapply ht_app); try eassumption. now apply ht_other2.
+  - set_unfold. intuition. subst.
+    repeat (eapply ht_app); eauto. now apply ht_other2.
+  - set_unfold. intuition.
+    repeat (eapply ht_app); eauto. now apply ht_other2.
+  - set_unfold. intuition. subst. econstructor.
+    + now apply ht_other2.
+    + has_type. eapply has_type_subst_last2; eauto.
+  - unfold wf_tm_set. intuition > [|econstructor].
+    + eapply has_type_lift2.
+      apply H0. apply tm_set_map_spec. eauto.
+    + now apply ht_other2.
+    + has_type. eapply has_type_fold2; try eassumption. apply H.
+  - set_unfold. intuition.
+    + eapply has_type_lift2. apply H0. left.
+      apply tm_set_map_spec. eauto.
+    + subst. econstructor > [now apply ht_other2|].
+      has_type. eapply has_type_fold2; auto. apply H.
+    + eapply has_type_lift2; eassumption.
+  - intuition. econstructor > [now apply ht_other2|].
+    has_type. eapply has_type_subst_last2; eauto.
+  - set_unfold. intuition. subst.
+    econstructor > [now apply ht_other2|].
+    has_type. eapply has_type_subst_last2; eauto.
+    now constructor.
+  - intuition. econstructor > [now apply ht_other2|].
+    has_type. eapply has_type_subst_last2; eauto.
+    now constructor.
+Qed.
+
+Theorem rl_wL C l m c :
+  [{ C; m --> c }] -> [{ C; l ∪ m --> c }].
+Proof.
+  revert C l m c.
+  assert (MU : forall C h l, tm_set_map (lift C) <{ h ∪ l }> ≡ (tm_set_map (lift C) h) ∪ (tm_set_map (lift C) l) ). {
+    intros C h1 h2 x. set_unfold. repeat (rewrite tm_set_map_spec).
+    set_unfold. split.
+    - intros [y [Hy ->]]. destruct Hy; ltac1:(intuition eauto).
+    - intros [[y [Hy ->]] | [y [Hy ->]]]; eauto.
+  }
+  intros * H. revert l.
+  induction H; intros h; try (rewrite union_assoc in *).
+  - now rewrite <- H.
+  - now apply rl_id.
+  - eapply rl_cut; eauto.
+  - apply rl_cL. specialize IHis_derivable with h.
+    now repeat (rewrite union_assoc in *).
+  - apply rl_botL.
+  - apply rl_topR.
+  - apply rl_orL; now rewrite <- union_assoc.
+  - now apply rl_orR1.
+  - now apply rl_orR2.
+  - apply rl_andL1; now rewrite <- union_assoc.
+  - apply rl_andL2; now rewrite <- union_assoc.
+  - now apply rl_andR.
+  - apply rl_impL > [easy|]. now rewrite <- union_assoc.
+  - apply rl_impR. now rewrite <- union_assoc.
+  - eapply rl_forL > [eassumption|].
+    now rewrite <- union_assoc.
+  - eapply rl_forR; try eassumption.
+    now rewrite MU.
+  - eapply rl_exL; try eassumption.
+    now rewrite MU, <- union_assoc.
+  - eapply rl_exR; eauto.
+  - eapply rl_nabL; try eassumption.
+    now rewrite <- union_assoc.
+  - eapply rl_nabR; eauto.
+Qed.
+
+Theorem is_derivable_wf_is_derivable C l c :
+  is_derivable_wf C l c -> [{ C; l --> c }].
+Proof.
+  intros DW. induction DW; subst.
+  - eapply rl_set; eassumption.
+  - rewrite <- union_empty. now apply rl_id.
+  - eapply rl_cut; try eassumption.
+    apply is_derivable_wf_wf in DW1. destruct DW1. assumption.
+  - now apply rl_cL.
+  - now apply rl_wL.
+  - rewrite <- union_empty. apply rl_botL.
+  - apply rl_topR.
+  - now apply rl_orL.
+  - now apply rl_orR1.
+  - now apply rl_orR2.
+  - now apply rl_andL1.
+  - now apply rl_andL2.
+  - now apply rl_andR.
+  - now apply rl_impL.
+  - now apply rl_impR.
+  - eapply rl_forL; eassumption.
+  - eapply rl_forR; eassumption.
+  - eapply rl_exL; eassumption.
+  - eapply rl_exR; eassumption.
+  - eapply rl_nabL; eassumption.
+  - eapply rl_nabR; eassumption.
+Qed.
+
+Theorem is_derivable_is_derivable_wf C l c :
+  wf_sequent C l c ->  [{ C; l --> c }] -> is_derivable_wf C l c.
+Proof.
+  intros [] D. unfold wf_tm_set in *. induction D; set_unfold.
+  - eapply wrl_set > [eassumption|].
+    apply IHD; set_solver.
+  - apply wrl_wL; try auto.
+    apply wrl_id; auto.
+  - eapply wrl_cut; first [apply IHD1 | apply IHD2]; set_solver.
+  - apply wrl_cL. apply IHD; set_solver.
+  - apply wrl_wL > [|apply wrl_botL]; set_solver.
+  - assert (E : l ≡ l ∪ ∅) > [set_solver|].
+    rewrite E. apply wrl_wL > [|apply wrl_topR].
+    clear E. set_solver.
+  - assert (is_form C <{b \/ d}>) by auto.
+    apply wrl_orL; first [apply IHD1 | apply IHD2];
+      intuition; subst; now has_type.
+  - apply wrl_orR1.
+    + now has_type.
+    + apply IHD; intuition. now has_type.
+  - apply wrl_orR2.
+    + now has_type.
+    + apply IHD; intuition. now has_type.
+  - assert (is_form C <{b /\ d}>) by auto.
+    apply wrl_andL1 > [now has_type|].
+    apply IHD; intuition. subst. now has_type.
+  - assert (is_form C <{b /\ d}>) by auto.
+    apply wrl_andL2 > [now has_type|].
+    apply IHD; intuition. subst. now has_type.
+  - assert (is_form C <{b /\ c}>) by auto. apply wrl_andR.
+    + apply IHD1. intuition. now has_type.
+    + apply IHD2. intuition. now has_type.
+  - assert (is_form C <{b > d}>) by auto. apply wrl_impL.
+    + apply IHD1. intuition. now has_type.
+    + apply IHD2; intuition. subst. now has_type.
+  - assert (is_form C <{b > c}>) by auto. apply wrl_impR.
+    apply IHD; intuition; subst; now has_type.
+  - eapply wrl_forL > [eassumption|].
+    apply IHD; intuition. subst.
+    eapply has_type_subst_last_s1 > [eassumption|].
+    assert (is_form C <{for T, b}>) by auto.
+    now has_type.
+  - eapply wrl_forR > [eassumption|].
+    apply IHD; intuition.
+    + apply tm_set_map_spec in H2 as [a [Ha1 Ha2]]. subst.
+      has_type. auto.
+    + apply has_type_fold2_2 > [apply H1|].
       now has_type.
-    - eapply wrl_forR > [eassumption|].
-      apply IHD; intuition.
-      + apply sq_set_map_spec in H2 as [a [Ha1 Ha2]]. subst.
-        has_type. auto.
-      + apply has_type_fold2_2 > [apply H1|].
-        now has_type.
-    - eapply wrl_exL > [eassumption|].
-      apply IHD; intuition.
-      + apply sq_set_map_spec in H3 as [a [Ha1 Ha2]]. subst.
-        has_type. auto.
-      + subst. apply has_type_fold2_2 > [apply H1|].
-        assert (is_form C <{ex T, b}>) by auto.
-        now has_type.
-      + now has_type.
-    - eapply wrl_exR > [eassumption|].
-      apply IHD; intuition.
-      eapply has_type_subst_last_s1 > [eassumption|].
+  - eapply wrl_exL > [eassumption|].
+    apply IHD; intuition.
+    + apply tm_set_map_spec in H3 as [a [Ha1 Ha2]]. subst.
+      has_type. auto.
+    + subst. apply has_type_fold2_2 > [apply H1|].
+      assert (is_form C <{ex T, b}>) by auto.
       now has_type.
-    - eapply wrl_nabL > [eassumption|].
-      apply IHD; intuition. subst.
-      eapply has_type_subst_last_s1.
-      + now apply ht_other.
-      + assert (is_form C <{nab T, b}>) by auto.
-        now has_type.
-    - eapply wrl_nabR > [eassumption|].
-      apply IHD; intuition.
-      eapply has_type_subst_last_s1.
-      + now apply ht_other.
-      + now has_type.
-  Qed.
+    + now has_type.
+  - eapply wrl_exR > [eassumption|].
+    apply IHD; intuition.
+    eapply has_type_subst_last_s1 > [eassumption|].
+    now has_type.
+  - eapply wrl_nabL > [eassumption|].
+    apply IHD; intuition. subst.
+    eapply has_type_subst_last_s1.
+    + now apply ht_other.
+    + assert (is_form C <{nab T, b}>) by auto.
+      now has_type.
+  - eapply wrl_nabR > [eassumption|].
+    apply IHD; intuition.
+    eapply has_type_subst_last_s1.
+    + now apply ht_other.
+    + now has_type.
+Qed.
 
 
-  Theorem nom_in_supp b T : exists a, ~ in_supp b (gtm_nom T a).
-  Proof. eexists. apply nom_fresh_in_supp. Qed.
+Theorem rl_nabL2 C T b l c :
+  exists2 n, ~ in_supp b (gtm_nom T n) &
+  (is_derivable C (l ∪ {[ subst_last C C (gtm_nom T n) b ]}) c ->
+  is_derivable C (l ∪ {[ <{nab T, b}> ]}) c).
+Proof.
+  exists (nom_fresh b).
+  - apply nom_fresh_in_supp.
+  - intros. eapply rl_nabL.
+    + apply nom_fresh_in_supp.
+    + eassumption.
+Qed.
 
-  Theorem rl_nabL2 C T b l c :
-    exists2 n, ~ in_supp b (gtm_nom T n) &
-    (is_derivable C (l ∪ {[ subst_last C C (gtm_nom T n) b ]}) c ->
-    is_derivable C (l ∪ {[ <{nab T, b}> ]}) c).
-  Proof.
-    exists (nom_fresh b).
-    - apply nom_fresh_in_supp.
-    - intros. eapply rl_nabL.
-      + apply nom_fresh_in_supp.
-      + eassumption.
-  Qed.
+(*
+Ltac rl_nabL n := edestruct rl_nabL2 as [n ?X ?H]; apply H; clear H.
+*)
 
-  Ltac rl_nabL n := edestruct rl_nabL2 as [n ?X ?H]; apply H; clear H.
+Theorem tm_set_swap (l : tm_set) a b :
+  <{ l +; a +; b }> ≡ <{ l +; b +; a }>.
+Proof. set_unfold. intuition. Qed.
 
-  Theorem sq_set_swap (l : sq_set) a b :
-    <{ l +; a +; b }> ≡ <{ l +; b +; a }>.
-  Proof. set_unfold. intuition. Qed.
+Theorem contrapositive C l b c :
+  [{ C ; l +; b --> c }] -> [{ C ; l +; ~ c --> ~ b }].
+Proof.
+  intros H.
+  apply rl_impR. rewrite tm_set_swap.
+  apply rl_impL; try assumption.
+  apply rl_botL.
+Qed.
 
-  Theorem contrapositive C l b c :
-    [{ C ; l +; b --> c }] -> [{ C ; l +; ~ c --> ~ b }].
-  Proof.
-    intros H.
-    apply rl_impR. rewrite sq_set_swap.
-    apply rl_impL; try assumption.
-    apply rl_botL.
-  Qed.
+Hint Rewrite in_supp_not : tm.
 
-  Theorem in_supp_not B n :
-    in_supp <{ ~ B }> n <-> in_supp B n.
-  Proof. unfold in_supp. simpl. intuition. Qed.
+Theorem rl_id2 C l t : is_derivable C (l ∪ {[t]}) t.
+Proof. intros. apply rl_id; easy. Qed.
 
-  Hint Rewrite in_supp_not : tm.
-
-  Theorem rl_id2 C l t :
-    is_derivable C (l ∪ {[t]}) t.
-  Proof. intros. apply rl_id; easy. Qed.
-
-  (*
-  Notation "({ C ; l --> c })" := (wf_sequent C l c -> is_derivable C l c)
-    (C custom stlc_ty, l custom stlc_tm, c custom stlc_tm) : stlc_scope.
-    *)
-
-  Theorem example1 C l T B :
-    [{ C ; l --> (∇ T, ~ B) ≡ ~ (∇ T, B) }].
-  Proof.
-    destruct (nom_in_supp B T) as [a Ha].
-    constructor; constructor.
-    - apply (rl_nabL a); tm_simpl.
-      { assumption. }
-      apply contrapositive. apply (rl_nabL a Ha).
-      apply rl_id2.
-    - apply (rl_nabR a); tm_simpl.
-      { assumption. }
-      apply contrapositive. apply (rl_nabR a Ha).
-      apply rl_id2.
-  Qed.
-
-  Theorem example2 C l T b c :
-    [{ C; l --> (∇ T, b \/ c) ≡ (∇ T, b) \/ (∇ T, c) }].
-  Proof.
-    destruct (nom_in_supp <{ b \/ c }> T) as [n Hn].
-    constructor; constructor.
-    - apply (rl_nabL n) > [easy|].
-      tm_simpl. apply rl_orL.
-      + apply rl_orR1. apply (rl_nabR n).
-        * unfold in_supp in *. simpl in *. intuition.
-        * apply rl_id2.
-      + apply rl_orR2. apply (rl_nabR n).
-        * unfold in_supp in *. simpl in *. intuition.
-        * apply rl_id2.
-    - apply (rl_nabR n) > [easy|].
-      tm_simpl. apply rl_orL.
-      + apply rl_orR1. apply (rl_nabL n).
-        * unfold in_supp in *. simpl in *. intuition.
-        * apply rl_id2.
-      + apply rl_orR2. apply (rl_nabL n).
-        * unfold in_supp in *. simpl in *. intuition.
-        * apply rl_id2.
-  Qed.
-End GLogic.
+(*
+Notation "({ C ; l --> c })" := (wf_sequent C l c -> is_derivable C l c)
+  (C custom stlc_ty, l custom stlc_tm, c custom stlc_tm) : stlc_scope.
+  *)
