theories/glogic_examples.v
@@ -1,0 +1,57 @@
+Require Export glogic.
+
+Theorem example1 C l T B :
+  [{ C ; l --> (∇ T, ~ B) ≡ ~ (∇ T, B) }].
+Proof.
+  destruct (nom_in_supp B T) as [a Ha].
+  constructor; constructor.
+  - apply (rl_nabL a); tm_simpl.
+    { assumption. }
+    apply contrapositive. apply (rl_nabL a Ha).
+    apply rl_id2.
+  - apply (rl_nabR a); tm_simpl.
+    { assumption. }
+    apply contrapositive. apply (rl_nabR a Ha).
+    apply rl_id2.
+Qed.
+
+Theorem example2 C l T b c :
+  [{ C; l --> (∇ T, b \/ c) ≡ (∇ T, b) \/ (∇ T, c) }].
+Proof.
+  destruct (nom_in_supp <{ b \/ c }> T) as [n Hn].
+  constructor; constructor.
+  - apply (rl_nabL n) > [easy|].
+    tm_simpl. apply rl_orL.
+    + apply rl_orR1. apply (rl_nabR n).
+      * unfold in_supp in *. simpl in *. intuition.
+      * apply rl_id2.
+    + apply rl_orR2. apply (rl_nabR n).
+      * unfold in_supp in *. simpl in *. intuition.
+      * apply rl_id2.
+  - apply (rl_nabR n) > [easy|].
+    tm_simpl. apply rl_orL.
+    + apply rl_orR1. apply (rl_nabL n).
+      * unfold in_supp in *. simpl in *. intuition.
+      * apply rl_id2.
+    + apply rl_orR2. apply (rl_nabL n).
+      * unfold in_supp in *. simpl in *. intuition.
+      * apply rl_id2.
+Qed.
+
+(*
+Theorem example3 C T t :
+  ~ [{ C; ∅ --> ∇ T, ∇ T, t 0 1 > ∇ T, t 0 0 }].
+Proof.
+  intros H.
+  remember <{ ∇ T, ∇ T, t 0 1 > (∇ T, t 0 0) }> as x. remember ∅ as e.
+  assert (E : e ≡ ∅) by (now (rewrite Heqe)).
+  clear Heqe.
+  induction H; subst.
+  - apply IHis_derivable.
+    + reflexivity.
+    + now rewrite H.
+  - set_solver.
+  - apply IHis_derivable1.
+    + assert (m ≡ ∅) by set_solver.
+      rewrite H2 in H1. inversion H1.
+      *)
